src/program_proof/rsm/distx_txnlog.v
@@ -23,17 +23,21 @@ Section program.
     | _ => True
     end.
   
-  Definition own_txnlog (log : loc) (gid : groupid) (γ : distx_names) : iProp Σ.
+  Definition is_txnlog (txnlog : loc) (gid : groupid) (γ : distx_names) : iProp Σ.
+  Admitted.
+
+  #[global]
+  Instance is_txnlog_persistent txnlog gid γ :
+    Persistent (is_txnlog txnlog gid γ).
   Admitted.
 
   Theorem wp_TxnLog__Lookup (log : loc) (lsn : u64) (gid : groupid) γ :
-    ⊢
-    {{{ own_txnlog log gid γ }}}
+    is_txnlog log gid γ -∗
+    {{{ True }}}
     <<< ∀∀ l, clog_half γ gid l >>>
       TxnLog__Lookup #log #lsn @ ↑txnlogN
     <<< ∃∃ l', clog_half γ gid l' >>>
     {{{ (c : command) (ok : bool) (pwrsS : Slice.t), RET (command_to_val pwrsS c, #ok);
-        own_txnlog log gid γ ∗
         own_pwrs_slice pwrsS c ∗
         ⌜if ok then l' !! (uint.nat lsn) = Some c else True⌝
     }}}.
@@ -44,12 +48,14 @@ Section program.
   Admitted.
 
   Theorem wp_TxnLog__SubmitAbort (log : loc) (ts : u64) (gid : groupid) γ :
-    ⊢
-    {{{ own_txnlog log gid γ }}}
+    is_txnlog log gid γ -∗
+    {{{ True }}}
     <<< ∀∀ vs, cpool_half γ gid vs >>>
       TxnLog__SubmitAbort #log #ts @ ↑txnlogN
     <<< cpool_half γ gid ({[CmdAbt (uint.nat ts)]} ∪ vs) >>>
-    {{{ (lsn : u64) (term : u64), RET (#lsn, #term); own_txnlog log gid γ }}}.
+    {{{ (lsn : u64) (term : u64), RET (#lsn, #term);
+        cmd_receipt γ gid (uint.nat lsn) (uint.nat term) (CmdAbt (uint.nat ts))
+    }}}.
   Proof.
     (*@ func (log *TxnLog) SubmitAbort(ts uint64) (uint64, uint64) {            @*)
     (*@     // TODO: marshalling a abort command                                @*)
@@ -59,12 +65,14 @@ Section program.
   Admitted.
 
   Theorem wp_TxnLog__SubmitCommit (log : loc) (ts : u64) (gid : groupid) γ :
-    ⊢
-    {{{ own_txnlog log gid γ }}}
+    is_txnlog log gid γ -∗
+    {{{ True }}}
     <<< ∀∀ vs, cpool_half γ gid vs >>>
       TxnLog__SubmitCommit #log #ts @ ↑txnlogN
     <<< cpool_half γ gid ({[CmdCmt (uint.nat ts)]} ∪ vs) >>>
-    {{{ (lsn : u64) (term : u64), RET (#lsn, #term); own_txnlog log gid γ }}}.
+    {{{ (lsn : u64) (term : u64), RET (#lsn, #term);
+        cmd_receipt γ gid (uint.nat lsn) (uint.nat term) (CmdCmt (uint.nat ts))
+    }}}.
   Proof.
     (*@ func (log *TxnLog) SubmitCommit(ts uint64) (uint64, uint64) {           @*)
     (*@     // TODO: marshalling a commit command                               @*)
@@ -74,14 +82,16 @@ Section program.
   Admitted.
 
   Theorem wp_TxnLog__SubmitPrepare
-    (log : loc) (ts : u64) (wrs : Slice.t)
-    (wrsM : dbmap) (gid : groupid) γ :
-    ⊢
-    {{{ own_txnlog log gid γ (* TODO: slice ownership *) }}}
+    (log : loc) (ts : u64) (pwrsS : Slice.t)
+    (pwrsL : list dbmod) (pwrs : dbmap) (gid : groupid) γ :
+    is_txnlog log gid γ -∗
+    {{{ own_dbmap_in_slice pwrsS pwrsL pwrs }}}
     <<< ∀∀ vs, cpool_half γ gid vs >>>
-      TxnLog__SubmitPrepare #log #ts (to_val wrs) @ ↑txnlogN
-    <<< cpool_half γ gid ({[CmdPrep (uint.nat ts) wrsM]} ∪ vs) >>>
-    {{{ (lsn : u64) (term : u64), RET (#lsn, #term); own_txnlog log gid γ }}}.
+      TxnLog__SubmitPrepare #log #ts (to_val pwrsS) @ ↑txnlogN
+    <<< cpool_half γ gid ({[CmdPrep (uint.nat ts) pwrs]} ∪ vs) >>>
+    {{{ (lsn : u64) (term : u64), RET (#lsn, #term);
+        cmd_receipt γ gid (uint.nat lsn) (uint.nat term) (CmdPrep (uint.nat ts) pwrs)
+    }}}.
   Proof.
     (* some mixcode bug when function takes a slice *)
     (*@     // TODO: marshalling a prepare command                              @*)
@@ -92,12 +102,14 @@ Section program.
 
   Theorem wp_TxnLog__SubmitRead
     (log : loc) (ts : u64) (key : string) (gid : groupid) γ :
-    ⊢
-    {{{ own_txnlog log gid γ }}}
+    is_txnlog log gid γ -∗
+    {{{ True }}}
     <<< ∀∀ vs, cpool_half γ gid vs >>>
       TxnLog__SubmitRead #log #ts #(LitString key) @ ↑txnlogN
     <<< cpool_half γ gid ({[CmdRead (uint.nat ts) key]} ∪ vs) >>>
-    {{{ (lsn : u64) (term : u64), RET (#lsn, #term); own_txnlog log gid γ }}}.
+    {{{ (lsn : u64) (term : u64), RET (#lsn, #term);
+        cmd_receipt γ gid (uint.nat lsn) (uint.nat term) (CmdRead (uint.nat ts) key)
+    }}}.
   Proof.
     (*@ func (log *TxnLog) SubmitRead(ts uint64, key string) (uint64, uint64) { @*)
     (*@     // TODO: marshalling a read command                                 @*)
@@ -108,12 +120,14 @@ Section program.
 
   Theorem wp_TxnLog__WaitUntilSafe
     (log : loc) (lsn : u64) (term : u64) (c : command) (gid : groupid) γ :
+    is_txnlog log gid γ -∗
     cmd_receipt γ gid (uint.nat lsn) (uint.nat term) c -∗
-    {{{ own_txnlog log gid γ }}}
+    {{{ True }}}
       TxnLog__WaitUntilSafe #log #lsn #term
     {{{ (ok : bool), RET #ok;
-        own_txnlog log gid γ ∗
-        ∃ l, clog_lb γ gid l ∧ ⌜l !! (uint.nat lsn) = Some c⌝
+        if ok
+        then ∃ l, clog_lb γ gid l ∧ ⌜l !! (uint.nat lsn) = Some c⌝
+        else True
     }}}.
   Proof.
     (*@ func (log *TxnLog) WaitUntilSafe(lsn uint64, term uint64) bool {        @*)
